app_verification_helpers.thy
@@ -1,0 +1,199 @@
+theory app_verification_helpers
+  imports 
+    program_verification_tactics
+    impl_language
+    crdt_specs2
+    unique_ids
+    program_proof_rules
+begin
+
+
+
+lemma use_some_wellFormed:
+  assumes e: "\<exists>some_generatedIds some_currentTransaction some_localState some_currentProc some_visibleCalls some_transactionStatus.
+       state_wellFormed
+        \<lparr>calls = s_calls', happensBefore = s_happensBefore', callOrigin = s_callOrigin',
+           transactionOrigin = s_transactionOrigin', knownIds = s_knownIds', invocationOp = s_invocationOp',
+           invocationRes = s_invocationRes', prog = progr, transactionStatus = some_transactionStatus,
+           generatedIds = some_generatedIds, localState = some_localState, currentProc = some_currentProc,
+           visibleCalls = some_visibleCalls, currentTransaction = some_currentTransaction\<rparr>"
+and R: "\<And>S. state_wellFormed S \<Longrightarrow> P S"
+shows "\<exists>some_generatedIds some_currentTransaction some_localState some_currentProc some_visibleCalls some_transactionStatus. 
+  P \<lparr>calls = s_calls', happensBefore = s_happensBefore', callOrigin = s_callOrigin',
+           transactionOrigin = s_transactionOrigin', knownIds = s_knownIds', invocationOp = s_invocationOp',
+           invocationRes = s_invocationRes', prog = progr, transactionStatus = some_transactionStatus,
+           generatedIds = some_generatedIds, localState = some_localState, currentProc = some_currentProc,
+           visibleCalls = some_visibleCalls, currentTransaction = some_currentTransaction\<rparr>"
+proof -
+  from e obtain some_generatedIds some_currentTransaction some_localState some_currentProc some_visibleCalls some_transactionStatus
+    where "state_wellFormed
+        \<lparr>calls = s_calls', happensBefore = s_happensBefore', callOrigin = s_callOrigin',
+           transactionOrigin = s_transactionOrigin', knownIds = s_knownIds', invocationOp = s_invocationOp',
+           invocationRes = s_invocationRes', prog = progr, transactionStatus = some_transactionStatus,
+           generatedIds = some_generatedIds, localState = some_localState, currentProc = some_currentProc,
+           visibleCalls = some_visibleCalls, currentTransaction = some_currentTransaction\<rparr>"
+    by blast
+  hence "P \<lparr>calls = s_calls', happensBefore = s_happensBefore', callOrigin = s_callOrigin',
+           transactionOrigin = s_transactionOrigin', knownIds = s_knownIds', invocationOp = s_invocationOp',
+           invocationRes = s_invocationRes', prog = progr, transactionStatus = some_transactionStatus,
+           generatedIds = some_generatedIds, localState = some_localState, currentProc = some_currentProc,
+           visibleCalls = some_visibleCalls, currentTransaction = some_currentTransaction\<rparr>"
+    by (rule R)
+  thus ?thesis
+    by blast
+qed
+
+lemma get_query_spec:
+  assumes wf: "\<exists>some_generatedIds some_currentTransaction some_localState some_currentProc some_visibleCalls some_transactionStatus.
+     state_wellFormed
+      \<lparr>calls = s_calls', happensBefore = s_happensBefore', callOrigin = s_callOrigin',
+         transactionOrigin = s_transactionOrigin', knownIds = s_knownIds', invocationOp = s_invocationOp',
+         invocationRes = s_invocationRes', prog = progr, transactionStatus = some_transactionStatus,
+         generatedIds = some_generatedIds, localState = some_localState, currentProc = some_currentProc,
+         visibleCalls = some_visibleCalls, currentTransaction = some_currentTransaction\<rparr>"
+    and upd_call: "s_calls' upd_c \<triangleq> Call oper upd_r"
+  shows "\<exists>ctxt. querySpec progr oper ctxt upd_r"
+proof -
+  from wf
+  obtain some_generatedIds some_currentTransaction some_localState some_currentProc some_visibleCalls some_transactionStatus
+    where state_wf: "state_wellFormed
+                  \<lparr>calls = s_calls', happensBefore = s_happensBefore', callOrigin = s_callOrigin',
+                     transactionOrigin = s_transactionOrigin', knownIds = s_knownIds', invocationOp = s_invocationOp',
+                     invocationRes = s_invocationRes', prog = progr, transactionStatus = some_transactionStatus,
+                     generatedIds = some_generatedIds, localState = some_localState, currentProc = some_currentProc,
+                     visibleCalls = some_visibleCalls, currentTransaction = some_currentTransaction\<rparr>"
+    by blast
+
+  from wf_queryspec[OF state_wf] upd_call
+  obtain ctxt where "querySpec progr oper ctxt upd_r"
+    apply atomize_elim
+    apply auto
+    by blast
+  thus ?thesis
+    by blast
+qed
+
+
+lemma query_result_undef:
+  assumes wf: "\<exists>some_generatedIds some_currentTransaction some_localState some_currentProc some_visibleCalls some_transactionStatus.
+     state_wellFormed
+      \<lparr>calls = s_calls', happensBefore = s_happensBefore', callOrigin = s_callOrigin',
+         transactionOrigin = s_transactionOrigin', knownIds = s_knownIds', invocationOp = s_invocationOp',
+         invocationRes = s_invocationRes', prog = progr, transactionStatus = some_transactionStatus,
+         generatedIds = some_generatedIds, localState = some_localState, currentProc = some_currentProc,
+         visibleCalls = some_visibleCalls, currentTransaction = some_currentTransaction\<rparr>"
+    and upd_call: "s_calls' upd_c \<triangleq> Call (Message (NestedOp (MessageId m) upd_op)) upd_r"
+    and upd_is_update: "is_update upd_op"
+  shows "upd_r = Undef"
+proof -
+
+  obtain ctxt where "querySpec progr (Message (NestedOp (MessageId m) upd_op)) ctxt upd_r"
+    using assms(1) get_query_spec upd_call by blast
+
+  thus "upd_r = Undef"
+    using upd_is_update
+    by (auto simp add: crdtSpec_def struct_field_def map_dw_spec_def map_spec_def messageStruct_def register_spec_def split: messageDataOp.splits registerOp.splits if_splits)
+
+qed
+
+
+lemma C_out_calls_remove_unaffected:
+  assumes "\<And>y. C_out y \<noteq> x"
+  shows "C_out_calls C_out (m(c := x)) vis
+  = C_out_calls C_out m vis - {c}"
+  using assms  by (auto simp add: C_out_calls_def)
+
+lemma C_out_nesting_simp:
+  assumes "C_out1 = C_out2 \<circ> f"
+  shows
+  "C_out_calls C_out1 op (C_out_calls C_out2 op vis)
+= C_out_calls C_out1 op vis" 
+  by (auto simp add: assms C_out_calls_def)
+
+lemma C_out_nesting_simp2[simp]:
+  shows
+  "C_out_calls (C_out \<circ> f) op (C_out_calls C_out op vis)
+= C_out_calls (C_out \<circ> f) op vis" 
+  by (auto simp add:  C_out_calls_def)
+
+lemma C_out_calls_empty[simp]: "C_out_calls C_out op {} = {}"
+  by (auto simp add: C_out_calls_def)
+
+lemma C_out_union: 
+"C_out_calls C_out op (A \<union> B) = C_out_calls C_out op A \<union> C_out_calls C_out op B"
+  by (auto simp add: C_out_calls_def)
+
+lemma C_out_insert: 
+"C_out_calls C_out op (insert c A) = (if \<exists>x. op c = C_out x then {c} else {}) \<union> C_out_calls C_out op A"
+  by (auto simp add: C_out_calls_def)
+
+lemma C_out_intersection: 
+"C_out_calls C_out op (A \<inter> B) = C_out_calls C_out op A \<inter> C_out_calls C_out op B"
+  by (auto simp add: C_out_calls_def)
+
+lemma C_out_minus: 
+"C_out_calls C_out op (A - B) = C_out_calls C_out op A - C_out_calls C_out op B"
+  by (auto simp add: C_out_calls_def)
+
+lemma in_C_out:
+"x \<in> C_out_calls C_out op vis
+\<longleftrightarrow> x\<in> vis \<and> (\<exists>y. op x = C_out y)"
+  by (auto simp add: C_out_calls_def)
+
+lemmas C_out_distrib = C_out_union  C_out_insert C_out_intersection C_out_minus
+
+
+
+
+
+lemma acyclic_updateHb1:
+  assumes "distinct cs"
+    and "vis \<inter> set cs = {}"
+  shows "acyclic (updateHb {} vis cs)"
+  using assms proof (induct cs arbitrary: vis)
+  case Nil
+  then show ?case by auto
+next
+  case (Cons a cs vis)
+  have "a \<notin> vis"
+    using Cons.prems(2) by auto
+
+
+  show ?case 
+    apply (simp add: updateHb_cons)
+    apply (subst updateHb_simp_split)
+  proof (rule acyclic_union_disjoint)
+    show "acyclic (vis \<times> {a})"
+      by (simp add: acyclic_prod `a \<notin> vis`)
+    show " acyclic (updateHb {} (insert a vis) cs)"
+    proof (rule Cons.hyps)
+      show "distinct cs"
+        using Cons.prems(1) by auto
+      show "insert a vis \<inter> set cs = {}"
+        using Cons.prems(1) Cons.prems(2) by auto
+    qed
+
+    show " snd ` updateHb {} (insert a vis) cs \<inter> fst ` (vis \<times> {a}) = {}"
+      using Cons.prems(2) snd_updateHb2 by fastforce
+  qed
+qed
+
+lemma acyclic_updateHb:
+  assumes "acyclic hb"
+    and "distinct cs"
+    and "vis \<inter> set cs = {}"
+    and "Field hb \<inter> set cs = {}"
+  shows "acyclic (updateHb hb vis cs)"
+  apply (subst  updateHb_simp_split)
+  using `acyclic hb`
+proof (rule acyclic_union_disjoint)
+
+  show "acyclic (updateHb {} vis cs)"
+    by (simp add: acyclic_updateHb1 assms(2) assms(3))
+
+  show "snd ` updateHb {} vis cs \<inter> fst ` hb = {}"
+    by (smt Domain_fst Field_def Int_iff assms(4) disjoint_iff_not_equal inf_sup_absorb snd_updateHb2 subset_eq)
+qed
+
+
+end
